Auto/Lib/OptionExtra.lean
@@ -4,4 +4,12 @@ namespace Auto
   | some a => p a
   | none   => True
 
+theorem Option.p_all_eq_true (p : α → Bool) (x : Option α) :
+  (x.all p = true) = Option.allp (fun x => p x = true) x :=
+  match x with
+  | .none => by
+    dsimp [Option.all, Option.allp]; simp
+  | .some x => by
+    dsimp [Option.all, Option.allp]
+
 end Auto
